theories/systemF_cbv_safety.v
@@ -1,0 +1,212 @@
+From Coq.Unicode Require Import Utf8.
+From Coq.Lists Require Import List.
+From Autosubst Require Import Autosubst.
+From Coq.Relations Require Import Relations.
+From Coq.micromega Require Import Lia.
+From ShortLogrels Require Import prelude language systemF_cbv.
+
+
+Definition rel_in_env (Δ : environment (expr → Prop)) (X : var) (v : expr) : Prop :=
+  is_val v ∧ match lookup Δ X with Some P => P v | None => True end.
+
+Fixpoint val_rel (Δ : environment (expr → Prop)) (τ : type) (v : expr) : Prop :=
+  match τ with
+  |TUnit => v = TT
+  |TVar X => rel_in_env Δ X v
+  |TProd τ1 τ2 => ∃ v1 v2, v = Pair v1 v2 ∧ val_rel Δ τ1 v1 ∧ val_rel Δ τ2 v2
+  |TFun τ1 τ2 => is_val v ∧ ∀ w, val_rel Δ τ1 w → Safe (val_rel Δ τ2) (App v w)
+  |TForAll τ => is_val v ∧ ∀ P, Safe (val_rel (P :: Δ) τ) (TApp v)
+  end.
+
+Definition expr_rel (Δ : environment (expr → Prop)) (τ : type) (e : expr) :=
+  Safe (val_rel Δ τ) e.
+
+Lemma val_rel_is_val Δ τ v : val_rel Δ τ v → is_val v.
+Proof.
+  revert Δ v; induction τ; intros Δ v; simpl in *; subst.
+  - intros ?; subst; constructor.
+  - intros Hv; apply Hv.
+  - firstorder; subst; constructor; eauto.
+  - tauto.
+  - intros Hv; eapply Hv.
+Qed.
+
+Lemma val_rel_weaken_gen Δ1 Δ' Δ2 τ v :
+  val_rel (Δ1 ++ Δ2) τ v ↔ val_rel (Δ1 ++ Δ' ++ Δ2) (weaken (length Δ1) (length Δ') τ) v.
+Proof.
+  revert Δ1 Δ' Δ2 v.
+  induction τ as [| X | | |]; intros Δ1 Δ' Δ2 v.
+  - simpl; tauto.
+  - simpl.
+    rewrite (@weaken_var type); [|apply _]; simpl.
+    unfold rel_in_env.
+    destruct Nat.ltb eqn:Hlt.
+    + apply PeanoNat.Nat.ltb_lt in Hlt.
+      repeat (rewrite lookup_app_l; [|assumption]).
+      tauto.
+    + apply PeanoNat.Nat.ltb_ge in Hlt.
+      rewrite app_assoc.
+      rewrite lookup_app_r; [|assumption].
+      rewrite lookup_app_r; [|rewrite app_length; lia].
+      rewrite app_length.
+      replace (X + length Δ' - (length Δ1 + length Δ')) with (X - length Δ1) by lia.
+      tauto.
+  - split; intros (?&?&?&?&?); eexists _, _; repeat split; eauto;
+      match goal with H : _ |- _ => apply H; eauto | H : _ |- _ => apply <- H; eauto end.
+  - split; intros [? Happ];
+      split; [assumption|intros; eapply Safe_mono; [intros|eapply Happ]|
+               assumption|intros; eapply Safe_mono; [intros|eapply Happ]];
+      match goal with H : _ |- _ => apply H; eauto | H : _ |- _ => apply <- H; eauto end.
+  - split; intros [? Htapp].
+    + split; [assumption|].
+      intros ?. eapply Safe_mono; [|eapply Htapp; fail].
+      intros ? ?.
+      apply (IHτ (_ :: _)); eassumption.
+    + split; [assumption|].
+      intros ?.
+      eapply Safe_mono; [|eapply Htapp; fail].
+      intros w Hw.
+      eapply (IHτ (_ :: _)) in Hw; eauto.
+Qed.
+
+Lemma val_rel_weaken Δ1 Δ2 τ v :
+  val_rel Δ2 τ v ↔ val_rel (Δ1 ++ Δ2) τ.[ren (+length Δ1)] v.
+Proof.
+  rewrite (val_rel_weaken_gen nil Δ1 Δ2); simpl.
+  rewrite weaken_0; asimpl; tauto.
+Qed.
+
+Lemma env_rel_weaken Δ1 Δ' Δ2 Γ env :
+  env_rel (val_rel (Δ1 ++ Δ2)) Γ env ↔
+    env_rel (val_rel (Δ1 ++ Δ' ++ Δ2)) (map (weaken (length Δ1) (length Δ')) Γ) env.
+Proof.
+  revert env.
+  induction Γ as [|τ Γ IHΓ]; intros env.
+  - split.
+    + intros ->%env_rel_inv_nil_l; apply env_rel_nil.
+    + intros ->%env_rel_inv_nil_l; apply env_rel_nil.
+  - split; simpl.
+    + intros (?&?&->&?&?)%env_rel_inv_cons_l.
+      apply env_rel_cons; [|apply IHΓ; eauto; fail].
+      apply val_rel_weaken_gen; auto.
+    + intros (?&?&->&?&?)%env_rel_inv_cons_l.
+      apply env_rel_cons; [|apply IHΓ; eauto; fail].
+      apply <- val_rel_weaken_gen; eauto.
+Qed.
+
+Lemma env_rel_weaken1 P Δ Γ env :
+  env_rel (val_rel Δ) Γ env → env_rel (val_rel (P :: Δ)) (map (rename (+1)) Γ) env.
+Proof. rewrite (env_rel_weaken (nil) (cons P nil) Δ); simpl; rewrite weaken_0; trivial. Qed.
+
+Lemma val_rel_subst_gen Δ1 τ' Δ2 τ v :
+  val_rel (Δ1 ++ (val_rel Δ2 τ') :: Δ2) τ v ↔ val_rel (Δ1 ++ Δ2) τ.[upn (length Δ1) (τ'.: ids)] v.
+Proof.
+  revert Δ1 Δ2 v.
+  induction τ as [| X | | |]; intros Δ1 Δ2 v.
+  - simpl; tauto.
+  - asimpl.
+    rewrite upn_ext.
+    destruct Nat.ltb eqn:Hlt.
+    + apply PeanoNat.Nat.ltb_lt in Hlt.
+      simpl; unfold rel_in_env; simpl.
+      repeat (rewrite lookup_app_l; [|assumption]); tauto.
+    + apply PeanoNat.Nat.ltb_ge in Hlt.
+      destruct (PeanoNat.Nat.eq_dec X (length Δ1)) as [->|].
+      * rewrite PeanoNat.Nat.sub_diag; asimpl.
+        unfold rel_in_env.
+        rewrite lookup_app_r; [|lia].
+        rewrite PeanoNat.Nat.sub_diag; simpl.
+        rewrite <- val_rel_weaken; intuition; eauto using val_rel_is_val.
+      * simpl; unfold rel_in_env; simpl.
+        rewrite lookup_app_r; [|lia].
+        destruct (X - length Δ1) as [|z] eqn:Heq; [lia|].
+        simpl; unfold rel_in_env; simpl.
+        rewrite lookup_app_r; [|lia].
+        replace (length Δ1 + z - length Δ1) with z by lia.
+        tauto.
+  - split; intros (?&?&?&?&?); eexists _, _; repeat split; eauto;
+      match goal with H : _ |- _ => apply H; eauto | H : _ |- _ => apply <- H; eauto end.
+  - split; intros [? Happ];
+      split; [assumption|intros; eapply Safe_mono; [intros|eapply Happ]|
+               assumption|intros; eapply Safe_mono; [intros|eapply Happ]];
+      match goal with H : _ |- _ => apply H; eauto | H : _ |- _ => apply <- H; eauto end.
+  - split; intros [? Htapp].
+    + split; [assumption|].
+      intros ?. eapply Safe_mono; [|eapply Htapp; fail].
+      intros ? ?.
+      apply (IHτ (_ :: _)); eassumption.
+    + split; [assumption|].
+      intros ?.
+      eapply Safe_mono; [|eapply Htapp; fail].
+      intros w Hw.
+      eapply (IHτ (_ :: _)) in Hw; eauto.
+Qed.
+
+Lemma val_rel_subst τ' Δ τ v : val_rel (val_rel Δ τ' :: Δ) τ v ↔ val_rel Δ τ.[τ'/] v.
+Proof. apply (val_rel_subst_gen nil). Qed.
+
+Theorem Fundamental Γ e τ :
+  typed Γ e τ → ∀ Δ env, env_rel (val_rel Δ) Γ env → expr_rel Δ τ e.[env_subst env].
+Proof.
+  intros Htp.
+  induction Htp; intros Δ env Henv; simpl.
+  - simpl.
+    assert (val_rel Δ τ (env_subst env v)).
+    { eapply env_rel_lookup1 in Henv as [? [? ?]]; [|eauto; fail].
+      erewrite env_subst_lookup; eauto. }
+    apply Safe_val; [eapply val_rel_is_val; eauto|assumption].
+  - apply Safe_val; [constructor|simpl; trivial].
+  - eapply (Safe_bind _ _ _ (λ e, Pair e _));
+      [repeat econstructor; fail|apply IHHtp1; eassumption; fail|].
+    intros v1 Hv11 Hv12.
+    eapply (Safe_bind _ _ _ (λ e, Pair _ e)); [|apply IHHtp2; eassumption; fail|].
+    { repeat econstructor; trivial. }
+    intros v2 Hv21 Hv22.
+    apply Safe_val; [constructor; trivial; fail|eexists _, _; eauto].
+  - eapply (Safe_bind _ _ _ (λ e, Fst e));
+      [repeat econstructor; fail|apply IHHtp; eassumption; fail|].
+    intros v Hv1 (v1 & v2 & -> & Hv1r & Hv2r).
+    inversion Hv1; subst.
+    eapply Safe_head_step_back; [solve_det_head_step|].
+    apply Safe_val; assumption.
+  - eapply (Safe_bind _ _ _ (λ e, Snd e));
+      [repeat econstructor; fail|apply IHHtp; eassumption; fail|].
+    intros v Hv1 (v1 & v2 & -> & Hv1r & Hv2r).
+    inversion Hv1; subst.
+    eapply Safe_head_step_back; [solve_det_head_step|].
+    apply Safe_val; assumption.
+  - apply Safe_val; [constructor; fail|].
+    split; [constructor; fail|].
+    intros w Hw.
+    assert (is_val w) by (eapply val_rel_is_val; eauto).
+    eapply Safe_head_step_back; [solve_det_head_step|].
+    asimpl.
+    apply (IHHtp Δ (_ :: _)).
+    apply env_rel_cons; assumption.
+  - eapply (Safe_bind _ _ _ (λ e, App e _));
+      [repeat econstructor; fail|apply IHHtp1; eassumption; fail|].
+    intros v1 Hv11 Hv12.
+    eapply (Safe_bind _ _ _ (λ e, App _ e)); [|apply IHHtp2; eassumption; fail|].
+    { repeat econstructor; trivial. }
+    intros v2 Hv21 Hv22.
+    apply Hv12; trivial.
+  - apply Safe_val; [constructor; fail|].
+    split; [constructor; fail|].
+    intros P.
+    eapply Safe_head_step_back; [solve_det_head_step|].
+    apply IHHtp.
+    apply env_rel_weaken1; trivial.
+  - eapply (Safe_bind _ _ _ (λ e, TApp e));
+      [repeat econstructor; fail|apply IHHtp; eassumption; fail|].
+    intros v ? [? Hv].
+    eapply Safe_mono; [|apply Hv; fail].
+    intros ? ?; rewrite <- val_rel_subst; eassumption.
+Qed.
+
+Corollary type_safety e τ : typed nil e τ → Safe (λ _, True) e.
+Proof.
+  intros Htp.
+  eapply Safe_mono; [tauto|].
+  replace e with e.[env_subst nil] by (asimpl; reflexivity).
+  eapply (Fundamental nil _ _ Htp nil); apply env_rel_nil.
+Qed.
